theories/scratch.v
@@ -1,0 +1,254 @@
+(* tid := nat
+obj : Type
+obj := loc * loc
+
+blocked : tid → option obj
+safe : obj → option tid
+
+(∃ t, blocked t = Some w) → is_Some (safe w)
+safe w = Some t → blocked t ≠ Some w
+blocked t = None → reducible (es !! i) *)
+
+From iris.proofmode Require Import tactics.
+
+Definition loc := nat.
+
+(*
+We have a heap of channel buffers indexed by loc's (e.g. natural numbers).
+We represent a channel as a pair of buffers.
+Each party will put its messages in one buffer and read from the other
+*)
+Definition chan := (loc * loc)%type.
+
+(*
+We have a lambda calculus-based language with natural numbers, closures, and unit.
+In addition we have channel values.
+*)
+Inductive val :=
+    | Unit : val
+    | Nat : nat -> val
+    | Pair : val -> val -> val
+    | Fun : string -> expr -> val
+    | Chan : chan -> val
+
+with expr :=
+    | Val : val -> expr
+    | Var : string -> expr
+    | App : expr -> expr -> expr
+    | Lam : string -> expr -> expr
+    | Send : expr -> expr -> expr
+    | Recv : expr -> expr
+    | Let : string -> expr -> expr -> expr
+    | LetUnit : expr -> expr -> expr
+    | LetProd : string -> string -> expr -> expr -> expr
+    | If : expr -> expr -> expr -> expr
+    | Fork : expr -> expr
+    | Close : expr -> expr.
+
+Definition state := gmap loc (list val).
+
+Inductive type :=
+    | UnitT : type
+    | NatT : type
+    | PairT : type -> type -> type
+    | FunT : type -> type -> type
+    | ChanT : chan_type -> type
+
+with chan_type :=
+    | SendT : type -> chan_type -> chan_type
+    | RecvT : type -> chan_type -> chan_type
+    | EndT : chan_type.
+
+Definition env := list (string * type).
+
+Fixpoint dual ct :=
+    match ct with
+    | EndT => EndT
+    | SendT c ct => RecvT c (dual ct)
+    | RecvT c ct => SendT c (dual ct)
+    end.
+
+Definition heapT := gmap chan chan_type.
+
+(* TODO: Add subscripts to vs code latex thing *)
+Definition disj_union (a b c : heapT) := a ##ₘ b ∧ c = a ∪ b.
+
+Inductive val_typed : heapT -> val -> type -> Prop :=
+    | Unit_typed :
+        val_typed ∅ Unit UnitT
+    | Nat_typed : forall n,
+        val_typed ∅ (Nat n) NatT
+    | Pair_typed : forall a b aT bT Σ Σ1 Σ2,
+        disj_union Σ Σ1 Σ2 ->
+        val_typed Σ1 a aT ->
+        val_typed Σ2 b bT ->
+        val_typed Σ (Pair a b) (PairT aT bT)
+    | Fun_typed : forall Σ x e a b,
+        typed Σ [(x,a)] e b ->
+        val_typed Σ (Fun x e) (FunT a b)
+    | Chan_typed : forall c ct,
+        val_typed {[ c := ct ]} (Chan c) (ChanT ct)
+
+with typed : heapT -> env -> expr -> type -> Prop :=
+    | Val_typed : forall Σ v t,
+        val_typed Σ v t ->
+        typed Σ [] (Val v) t
+    | Var_typed : forall x t,
+        typed ∅ [(x,t)] (Var x) t
+    | App_typed : forall Σ Σ1 Σ2 Γ Γ1 Γ2 e1 e2 t1 t2,
+        disj_union Σ Σ1 Σ2 ->
+        Γ ≡ₚ Γ1 ++ Γ2 ->
+        typed Σ1 Γ1 e1 (FunT t1 t2) ->
+        typed Σ2 Γ2 e2 t1 ->
+        typed Σ Γ (App e1 e2) t2
+    | Lam_typed : forall Σ Γ x e t1 t2,
+        typed Σ ((x,t1)::Γ) e t2 ->
+        typed Σ Γ (Lam x e) (FunT t1 t2)
+    | Send_typed : forall Σ Σ1 Σ2 Γ Γ1 Γ2 e1 e2 t r,
+        disj_union Σ Σ1 Σ2 ->
+        Γ ≡ₚ Γ1 ++ Γ2 ->
+        typed Σ1 Γ e1 (ChanT (SendT t r)) ->
+        typed Σ2 Γ e2 t ->
+        typed Σ Γ (Send e1 e2) (ChanT r)
+    | Recv_typed : forall Σ Γ e t r,
+        typed Σ Γ e (ChanT (RecvT t r)) ->
+        typed Σ Γ (Recv e) (PairT t (ChanT r))
+    | Let_typed : forall Σ Σ1 Σ2 Γ Γ1 Γ2 e1 e2 t1 t2 x,
+        disj_union Σ Σ1 Σ2 ->
+        Γ ≡ₚ Γ1 ++ Γ2 ->
+        typed Σ1 Γ1 e1 t1 ->
+        typed Σ2 ((x,t1)::Γ2) e2 t2 ->
+        typed Σ Γ (Let x e1 e2) t2
+    | If_typed : forall Σ Σ1 Σ2 Γ Γ1 Γ2 e1 e2 e3 t,
+        Γ ≡ₚ Γ1 ++ Γ2 ->
+        disj_union Σ Σ1 Σ2 ->
+        typed Σ1 Γ1 e1 NatT ->
+        typed Σ2 Γ2 e2 t ->
+        typed Σ2 Γ2 e3 t ->
+        typed Σ Γ (If e1 e2 e3) t
+    | Fork_typed : forall Σ Γ e ct,
+        typed Σ Γ e (FunT (ChanT (dual ct)) UnitT) ->
+        typed Σ Γ (Fork e) (ChanT ct)
+    | Close_typed : forall Σ Γ e,
+        typed Σ Γ e (ChanT EndT) ->
+        typed Σ Γ (Close e) UnitT.
+
+(* FIXME: implement substitution *)
+Definition subst (x:string) (a:val) (e:expr) : expr := Val Unit.
+
+Inductive head_step : expr -> state -> expr -> state -> Prop :=
+    | App_head_step : forall x e s a,
+        head_step (App (Val (Fun x e)) (Val a)) s (subst x a e) s
+    | Lam_head_step : forall x e s,
+        head_step (Lam x e) s (Val (Fun x e)) s
+    | Let_head_step : forall x v e2 s,
+        head_step (Let x (Val v) e2) s (subst x v e2) s
+
+    (* Not clear how to do this... *)
+    | Send_head_step : forall s l1 l2 y buf,
+        s !! l1 = Some buf ->
+        head_step (Send (Val (Chan (l1,l2))) (Val y)) s (Val (Chan (l1,l2))) (<[l1 := y::buf]> s)
+    | Recv_head_step : forall s l1 l2 y buf,
+        s !! l2 = Some (y :: buf) ->
+        head_step (Recv (Val (Chan (l1,l2)))) s (Val (Pair (Chan (l1,l2)) y)) (<[l2 := buf]> s)
+
+    | If_head_step1 : forall n s e1 e2,
+        n ≠ 0 ->
+        head_step (If (Val (Nat n)) e1 e2) s e1 s
+    | If_head_step2 : forall s e1 e2,
+        head_step (If (Val (Nat 0)) e1 e2) s e1 s
+
+    (* TODO: implement these steps *)
+    | LetUnit_head_step : forall e s, head_step e s e s
+    | LetProd_head_step : forall e s, head_step e s e s
+    | Close_step : forall l1 l2 s,
+        head_step (Close (Val (Chan (l1,l2)))) s (Val Unit) (delete l1 s).
+        (* TODO: check whether it matters that we delete l1 s here *)
+
+(* We put the fork step here because it needs to spawn a new thread. *)
+(* FIXME step under contexts
+    Build contexts into these rules *)
+Inductive step : list expr -> state -> list expr -> state -> Prop :=
+    | Head_step : forall e1 e2 s1 s2 es i,
+        head_step e1 s1 e2 s2 ->
+        es !! i = Some e1 ->
+        step es s1 (<[i := e2]> es) s2
+    | Fork_step : forall (es : list expr) i e (s : state) e1 (l1 l2 : loc),
+        es !! i = Some (Fork e) ->
+        s !! l1 = None ->
+        s !! l2 = None ->
+        l1 ≠ l2 ->
+        step e1 s
+            (<[i := Val Unit]> e1 ++ [App e (Val (Chan (l1,l2)))])
+            (<[l1 := []]> $ <[l2 := []]> s).
+
+(* Closure of the step relation; this is used in the theorem statement. *)
+Inductive steps : list expr -> state -> list expr -> state -> Prop :=
+    | Trans_step : forall e1 e2 e3 s1 s2 s3,
+        step e1 s1 e2 s2 ->
+        steps e2 s2 e3 s3 ->
+        steps e1 s1 e3 s3
+    | Empty_step : forall e1 s1,
+        steps e1 s1 e1 s1.
+
+Inductive all_values : list expr -> Prop :=
+    | AV_nil : all_values []
+    | AV_cons : forall es v, all_values es -> all_values (Val v :: es).
+
+Definition disjoint (xs : list heapT) := True.
+
+Definition invariant (es : list expr) (s : state) : Prop :=
+(*
+    This invariant should make sure that either all es are values or some e in es can take a step.
+    We need to ensure that the expr and state are well typed.
+    And we need to ensure that we have an acyclic connectivity graph.
+    Picture the current state as a graph with threads as vertices.
+    The vertices are connected by channels, so each edge stores a channel.
+    A channel consists of a pair of buffers and a channel type for each endpoint.
+    The channel types are dual up to what is already stored in the buffer.
+    The connectivity graph must be acyclic.
+*)
+    Forall2 (λ Σ e, typed Σ ∅ e UnitT) Σs es ∧ disjoint Σs.
+    (* TODO: figure out invariant
+        * Maintain graph + acyclicity predicate
+        * Or maintain Coq tree with tree rotations/surgery
+     *)
+
+Theorem invariant_init e : invariant [e] [].
+
+Theorem invariant_step e1 s1 e2 s2 :
+    invariant e1 s1 ->
+    step e1 s1 e2 s2 ->
+    invariant e2 s2.
+(*
+    For steps not involving channels, we need to ensure that they preserve types.
+    The interesting steps are fork, send, recv.
+
+    Fork creates a new thread in the connectivity graph. The parent thread gives some of its linear resources to
+    the forked thread. Finally, we insert an edge between the forked thread and the parent thread, which has a
+    channel with dual session types and empty buffers. So this preserves the invariant.
+
+    Send takes a linear resource from a thread and puts it in one of the buffers of a channel endpoint that
+    the thread owns. This simultaneously steps the session protocol and puts something in the buffer. So this
+    preserves the invariant.
+
+    Receive takes an element out of one of the channel endpoints that the thread owns. This simultaneously steps
+    the session protocol and takes something out of the buffer. So this preserves the invariant.
+*)
+
+Theorem deadlock_freedom e e1 s1 :
+    steps [e] [] e1 s1 ->
+    all_values e1 ∨ exists e2 s2, step e1 s1 e2 s2.
+(*
+    We first check if all threads are values. If so, we return the first disjunct.
+    If there is a thread that's not a value, we will start an iterative process.
+    If the thread is not blocked on receive, we are done, because then the thread can take a step.
+    If it is blocked on receive, we look at which channel it is blocked on, and to which thread
+    the other endpoint is connected to. We continue the iterative process at that thread.
+    Because the connectivity graph is a tree, this process will not go in a cycle, so it eventually
+    terminates at a thread that can take a step.
+
+    The crucial point is that it is never the case that two threads connected to a channel c are
+    both blocked on c. Therefore this iterative process never goes back to where it came from.
+    Instead it follows some path in an acyclic graph, and since the graph is finite this will terminate.
+*)
